



How symmetric can a function be?

D.C. van Leijenhorst¹

*Department of Mathematics, University of Nijmegen, Toernooiveld 1, 6525 ED Nijmegen,
The Netherlands*

Received 15 October 1997; received in revised form 6 February 1998; accepted 17 February 1998

Submitted by R.A. Brualdi

Abstract

The symmetric complexity of a polynomial f in n variables is defined as the number of times the fundamental theorem on symmetric functions is applicable. In this paper a sharp upper bound on this measure is derived by a matrix method. © 1998 Elsevier Science Inc. All rights reserved.

Keywords: Symmetric functions; Complexity; Term orderings; Recursions; Matrix spectra

1. Introduction

Consider a field K of characteristic 0, and let R be the ring $K[x_1, \dots, x_n]$ where n is > 0 .

A *symmetric function* is any element of R invariant under the symmetric group acting as coordinate permutations. Examples are the *elementary symmetric functions*: $a_0 = 1$, $a_i = \sum_{1 \leq j_1 < j_2 < \dots < j_i \leq n} x_{j_1} x_{j_2} \dots x_{j_i}$ ($1 \leq i \leq n$); $a_i = 0$ ($i < 0$ or $i > n$).

The *Fundamental Theorem on Symmetric Functions* [1,2] states that any symmetric function f can be uniquely written as $g(a_1, \dots, a_n)$ for some $g = g(x_1, \dots, x_n)$ from R , called the *symmetric representation* of f .

The symmetric functions are beautiful objects with a large algebraic-combinatorial theory [1]. By the above theorem they are the result of the substitution

¹ E-mail: bolke@cs.kun.nl.

$\sigma : g(x_1, \dots, x_n) \rightarrow g(a_1, \dots, a_n)$ that maps R isomorphically onto a smaller subring. Inspired by this fact and by the recent interest in fractals and dynamical systems ([3]), one might be curious about those polynomials that are obtained by iterating σ .

One question to ask in this context is of course, how to find fixpoints (if any). Here however, we shall restrict ourselves to a small numerical example in Section 5 because we wish to look at the matter from the perspective of complexity theory.

Definition 1. A polynomial f in n variables is 0-fold symmetric if f is not symmetric; and k -fold symmetric with $k > 0$ if f is symmetric and the symmetric representation of f is $(k - 1)$ -fold symmetric. The number k is called the *symmetric complexity* of f .

A k -fold symmetric function f possesses a high degree of symmetry indeed, and it seems an interesting complexity problem to find a bound on the natural measure k , expressed in the coefficients and exponents of f . Such a result will be given in the corollary to Theorem 1.

Equivalently, from an algorithmic point of view, any implementation of the fundamental theorem on symmetric functions can be seen as an abstract machine of which one might ask if and when it will halt on repeated action from a given input. In fact, the problem of this article arose from a study of efficient computer algebra implementations of this theorem.

Our method is based on term orderings and the like, familiar from Groebner basis theory [4]. Thus it is possible to translate the problem into linear algebra, involving the explicit calculation of the spectrum and eigenvectors of a matrix.

As an addendum to this paper, some Maple code can be found on the WWW at <http://www.cs.kun.nl/bolke/ksymmaple>.

2. Notations and generalities

Set $\mathbf{x} = (x_1, \dots, x_n)$. Let $a_i = a_i(\mathbf{x})$ be defined as above, and $\mathbf{a} = (a_1, \dots, a_n)$. Stretching notation a bit, we can view $\{c_1, \dots, c_n\} \rightarrow \mathbf{a}(\mathbf{c})$ as a mapping from the unordered lists of length n over K to K^n , which is a bijection if K is algebraically closed. Indeed, one has $\sum_{i=0}^n a_i(c_1, \dots, c_n)T^i = \prod_{i=1}^n (c_i T + 1)$. Instead of this however we shall consider the simpler mappings $\mathbf{c} \rightarrow \mathbf{a}(\mathbf{c})$ from K^n to K^n and $a : \mathbf{x} \rightarrow a(\mathbf{x})$ from R to R .

Definition 2. Let $\mathbf{a}^0 = (x_1, \dots, x_n)$ and for $k > 0$ define $\mathbf{a}^k = (a_1^k, a_2^k, \dots, a_n^k)$, where $a_i^k = a_i^k(\mathbf{x}) = a_i(a_1^{k-1}, a_2^{k-1}, \dots, a_n^{k-1})$, $1 \leq i \leq n$.

The a_i^k are called the *iterated elementary symmetric functions* (iesf's.). An interesting fact is given by

Lemma 1. For all $k \geq 1$, the iesf's $a_1^k, a_2^k, \dots, a_n^k$ are algebraically independent.

Proof. Induction w.r.t. k . For $k = 1$ this is well-known [2]. Now let $f(y_1, \dots, y_n)$ be such that $f(a_1^{k+1}, a_2^{k+1}, \dots, a_n^{k+1}) = 0$ in R .

By definition of the a_i^k 's, there exists a symmetric polynomial $g(z_1, \dots, z_n) = f(a_1(z), a_2(z), \dots, a_n(z))$ with $g(a_1^k, a_2^k, \dots, a_n^k) = f(a_1^{k+1}, a_2^{k+1}, \dots, a_n^{k+1}) = 0$; hence $g(z_1, \dots, z_n) = 0$ by the induction hypothesis. But now we are in the case $k = 1$ again, since $g(z_1, \dots, z_n) = f(a_1(z), a_2(z), \dots, a_n(z))$ and it follows that $f(y_1, \dots, y_n) = 0$. \square

A *term* is any monomial $t = x_1^{i_1} x_2^{i_2} \dots x_n^{i_n}$. Its *total degree* is $\text{tdeg}(t) = \sum_{j=1}^n i_j$ and the total degree $\text{tdeg}(f)$ of $f \in R$ is $\max_{t \in f} \text{tdeg}(t)$ (which of course is equal to $\text{tdeg}(t)$, any t in f if f is symmetric.)

An *admissible ordering* [4] on the set T of terms in R is a total order on T that satisfies:

$$1 < t \quad \text{and} \quad t < t' \Rightarrow st < st' \quad \text{for all terms } s, t, t'.$$

The latter property is called *monotonicity* of term multiplication.

An admissible ordering is a well-ordering. Admissible orders abound and have been classified; well-known examples are the lexicographic orders and various total degree orderings like the “grevlex” [4].

For a given ordering, the *leading term* $\text{lt}(f)$ of f is the highest term occurring in f .

3. Main results

As an admissible ordering on T , let us take the lexicographic order with $x_1 > x_2 > \dots > x_n$.

Definition 3. The exponents (column) vector $\text{ev}(t)$ of a term $t = x_1^{i_1} \dots x_n^{i_n}$ is $\mathbf{i} = (i_1, i_2, \dots, i_n)^T$.

Definition 4. The term $\text{lt}(a_i^k)$ ($i \geq 1$) will be denoted by t_i^k , and $\text{ev}(t_i^k)$ by $\mathbf{e}_i^k = (e_{i,1}^k, \dots, e_{i,n}^k)^T$.

Our first result is the following.

Theorem 1. Let U be the upper triangular all-one matrix and D the (symmetric) lower antitriangular all-one matrix. Then for any k -fold symmetric function f and $k \geq 1$,

$$\text{ev}(\text{lt}(f)) \in UD^{k-1}((\mathbb{N} \cup \{0\})^n).$$

A reasonable way to get a grip on the entries of D^k is via the eigenvalues of D . The eigenvalue computation will be done in Section 4.1 and the entries of D^k will be estimated in Section 4.2. As a consequence, we have

Corollary 1. *Let f be any nonconstant k -fold symmetric polynomial in $n \geq 2$ variables. Then the symmetric complexity k is bounded by*

$$\text{tdeg}(f) \geq \frac{(2n+1)^{k-1}}{\pi^{k-1}} \{1.149 - 1.048(0.53)^{k-1}\}.$$

Remark 1. This bound is fairly precise: it is an approximation of a more complex bound, which is sharp in the sense that it is reached by $f = a_1^k$. This will follow from the proof.

Let us give an outline first. The idea is very simple and consists of three steps.

(i) If k increases, one observes that the iesf's a_i^k grow very quickly in “size” (explicit calculation of the complete a_i^k 's in Maple, say, leads to considerable memory problems). To measure this size, we consider the highest terms t_i^k of a_i^k in the chosen admissible ordering, and derive a recursion for the exponents occurring in this terms.

(ii) Next, for a given f of symmetric complexity k we shall show that some term t_i^k actually occurs in f as $\text{lt}(f)$. This proves Theorem 1 and shows that k is bounded as a function of $\text{lt}(f)$.

(iii) Finally, we shall be able to estimate the exponents occurring in $\text{lt}(f)$; this is the technical part of Section 4.

3.1. Proof of Theorem 1

We shall start with a recursion for t_i^k .

Lemma 2. (a) $t_i^k = t_n^{k-1} t_{n-1}^{k-1} \dots t_{n-i+1}^{k-1}$ ($k > 1$). (b) If $p > q$, $t_p^k > t_q^k$ ($k \geq 1$).

Proof. For $k = 1$, statement (b) holds. Indeed, $t_i^1 = \text{lt}(a_i) = x_1 x_2 \dots x_i$. Also, (a) holds trivially. Now if for any k (a) and (b) are true, then by definition one has $a_i^{k+1} = \sum_{1 \leq j_1 < j_2 < \dots < j_k \leq n} a_{j_1}^k a_{j_2}^k \dots a_{j_k}^k$. All coefficients are positive, so no terms cancel. By the monotonicity property, $\text{lt}(a_{j_1}^k a_{j_2}^k \dots a_{j_k}^k) = \text{lt}(a_{j_1}^k) \text{lt}(a_{j_2}^k) \dots \text{lt}(a_{j_k}^k) = t_{j_1}^k t_{j_2}^k \dots t_{j_k}^k$. Since (b) holds and, again, by monotonicity, this is maximal if $j_i = n$, $j_{i-1} = n-1, \dots, j_1 = n-i+1$. This proves (a) for index $k+1$. But then, if $p > q$ one has $t_p^{k+1} > t_q^{k+1}$ since the r.h.s. divides the l.h.s. Hence (b) holds as well. \square

Now consider $\text{ev}(t_i^k) = \mathbf{e}_i^k = (e_{i,1}^k, \dots, e_{i,n}^k)^T$ (see Definition 4). Define E_k to be the matrix having the \mathbf{e}_i^k 's as its columns. One has $\mathbf{e}_i^1 = (1, 1, \dots, 1, 1, 0, \dots, 0)^T$ (i ones), so $E_1 = U$.

Lemma 3. (a) Let $t = x_1^{i_1} \dots x_n^{i_n}$ be any term; then for all $k \geq 1$ the exponents vector of $\text{lt}(t(a_1^k, \dots, a_n^k))$ equals $E_k \mathbf{i}$.

(b) Let D be the symmetric matrix with ones below and on the antidiagonal and zeroes above. Let U be the upper triangular all-one matrix. Then $E_k = UD^{k-1}$. Hence E_k is nonsingular and for $k \geq 1$, $1 \leq a \leq n$ one has $\mathbf{e}_{i,a}^k = \sum_{j=i}^n (D^{k-1})_{j,a}$.

Proof. By monotonicity, $\text{lt}((a_1^k)^{i_1} \dots (a_n^k)^{i_n}) = (t_1^k)^{i_1} \dots (t_n^k)^{i_n}$, the exponents vector of which is $E_k \mathbf{i}$ by linearity. This proves part (a).

For part (b), note that statement (a) of Lemma 2 can be written as: $\mathbf{e}_i^k = \mathbf{e}_n^{k-1} + \mathbf{e}_{n-1}^{k-1} + \dots + \mathbf{e}_{n-i+1}^{k-1}$, which is equivalent to $E_k = E_{k-1}D$. So $E_k = E_1 D^{k-1} = UD^{k-1}$. \square

This is step i of the outline. In Section 4.1 we shall find an explicit solution to this recursion.

Now consider step ii. Suppose that f is not constant and k -fold symmetric, $k \geq 1$. We wish to prove that some t_i^k actually occurs in f .

By definition, there exists $f_k \in R$ such that $f_k(a_1^k, \dots, a_n^k) = f$ (though we shall not need it, note that f_k is unique by Lemma 1). Let $t = x_1^{i_1} \dots x_n^{i_n}$ be a term of the polynomial $f_k(\mathbf{x})$ such that $\tau =_{\text{Def}} \text{lt}((a_1^k)^{i_1}, \dots, (a_n^k)^{i_n})$ is *maximal* in the term ordering. By Lemma 3, $\text{ev}(\tau) = E_k(i_1, \dots, i_n)^T = E_k \mathbf{i}$.

First note that τ is unique. Indeed, suppose that besides t there is another term $s = x_1^{j_1} \dots x_n^{j_n}$ yielding the same τ , then by Lemma 3 one would have $E_k \mathbf{i} = E_k \mathbf{j}$ (with $\mathbf{j} = (j_1, \dots, j_n)^T$); hence $E_k(\mathbf{i} - \mathbf{j}) = \mathbf{0}^T$. But E_k was nonsingular so $\mathbf{i} = \mathbf{j}$ and $s = t$.

Also, τ does not cancel when $f_k(a_1^k, \dots, a_n^k)$ is expanded to f . Otherwise, there would be some term s in f_k and a term σ from $s(a_1^k, \dots, a_n^k)$ such that $\tau = \sigma$. (Note: all these terms are in R , i.e. of the form $x_1^{p_1} \dots x_n^{p_n}$.) Then however, $\sigma \leq \text{lt}(s(a^k)) < \text{lt}(t(a^k))$. This contradicts the unicity of t and the maximality of τ .

We conclude that $\tau = \text{lt}(f)$. This shows what we wanted, namely that some t_i^k occurs in t , hence in f . \square

In fact we have implicitly proven Theorem 1.

4. The size of the exponents

How good is Theorem 1? In order to answer this question let us give an estimate of the entries of powers of D . As stated in the introduction, a good way to do this is by looking at the eigenvalues.

A matrix like D has been used before by Raney [6] in a completely different context. In his paper [5], he considers a matrix Q_n equivalent to D by reversal of the order of the coordinates, and the dominant eigenvalue and its eigenvector are computed. Though his result is in principle applicable to estimate $\text{tdeg}(f)$ asymptotically, we shall by a different procedure be able to find the complete spectrum of D with its eigenvector basis, obtain a more precise estimate for $\text{tdeg}(f)$, and, moreover, derive an explicit formula in closed form for D^k .

4.1. The eigenvectors of D

For $p = 1, 2, \dots, n$, let us define the following quantities:

$$w_p = -\exp\left(\frac{-2p\pi i}{2n+1}\right);$$

$$\alpha_p = w_p + w_p^{-1} = -2 \cos\left(\frac{2p\pi}{2n+1}\right); \quad V_p = w_p - w_p^{-1} = 2i \sin\left(\frac{2p\pi}{2n+1}\right);$$

$$\lambda_p = 4 \cos^2\left(\frac{p\pi}{2n+1}\right); \quad \mu_p = (-1)^n / 2 \cos\left(\frac{2p\pi}{2n+1}\right);$$

$$x_m^p = 2(-1)^{m+1} \frac{\sin(2pm\pi/2n+1)}{\sqrt{2n+1}} \quad (m = 1, 2, \dots, n);$$

$$\mathbf{x}^p = (x_1^p, x_2^p, \dots, x_n^p).$$

These numbers satisfy the relations:

$$\lambda_p = 2 + \alpha_p; \quad V_p^2 = \alpha_p^2 - 4; \quad w_p^{2n+1} = -1; \quad \mu_p = \frac{1}{(w_p^n + w_p^{-n})};$$

$$\mu_p^{-2} = \lambda_p; \quad x_m^p = \frac{(w_p^m - w_p^{-m})}{i\sqrt{2n+1}} \quad (m = 1, 2, \dots, n);$$

also, $w_p = (\alpha_p + V_p)/2$ and $w_p^{-1} = (\alpha_p - V_p)/2$ are the roots of $X^2 - \alpha_p X + 1 = 0$.

Let $\langle \mathbf{x}, \mathbf{y} \rangle = \sum_{i=1}^n x_i \bar{y}_i$ be the standard Hermitian inner product. It is elementary to verify that the \mathbf{x}_p are perpendicular of length 1. Now one has the following.

Proposition 1. *The vectors \mathbf{x}_p form an orthonormal basis upon which the matrix D assumes a diagonal form $\Delta = \text{Diag}(\mu_1, \mu_2, \dots, \mu_n)$.*

Proof. Since the proof is fairly standard, let us just outline it. Instead of working with D (like in [5]) we shall first diagonalize D^{-2} , which is much easier.

Indeed, one readily verifies that the inverse of D is the matrix with ones on the antidiagonal, -1 's just above it, and zeroes elsewhere. Next, its square D^{-2} is seen to be tridiagonal: $(D^{-2})_{i,i} = 2$ ($i < n$); $(D^{-2})_{n,n} = 1$; $(D^{-2})_{i,j} = -1$ ($|i - j| = 1$).

Tridiagonal matrices have been studied extensively in the theory of orthogonal polynomials [6] and the numerical theory of parabolic differential equations.

D^{-2} , being symmetric, can be diagonalized on a real orthonormal basis. Let $\mathbf{z} = (z_1, z_2, \dots, z_n)$ be an eigenvector of D^{-2} with eigenvalue λ . Put $\mathbf{z} = \mathbf{z}(\alpha)$, again with $\alpha = 2 - \lambda$. W.l.o.g, let $z_1 = 1$ and $z_0 =_{\text{Def}} 0$. Then $(D^{-2} - \lambda I)\mathbf{z}^T = \mathbf{0}^T$ amounts to the recursion

$$\begin{aligned} z_0 &= 0; & z_1 &= 1; & z_m &= \alpha z_{m-1} - z_{m-2} \quad (1 < m \leq n); \\ & & & & -z_{n-1} &+ (\alpha - 1)z_n = 0 \end{aligned}$$

(the latter being the characteristic equation).

Remark 2. This is the familiar recursion of the Tchebycev polynomials $T_{m-1}(x)$ in $x = \alpha/2$, though these have initial values $T_0 = 1$, $T_1 = x$. In fact it is not difficult to prove that

$$z_m = \frac{((\alpha/2)T_m(\alpha/2) - T_{m-1}(\alpha/2))}{((\alpha/2)^2 - 1)}.$$

Let $V = \sqrt{\alpha^2 - 4}$ and $w = (\alpha + V)/2$, $w' = (\alpha - V)/2$, the roots of $X^2 - \alpha X + 1 = 0$. If $w = w'$, $\alpha = \pm 2$; but then $z_m = (\pm 1)^{m-1}m$, $-z_{n-1} + (\alpha - 1)z_n \neq 0$, and there are no eigenvalues. So suppose $w \neq w'$.

Solving the recursion by standard techniques yields $z_m = (w^m - w'^m)/V$; $1 \leq m \leq n$. By some easy calculations, the eigenvalue equation $-z_{n-1} + (\alpha - 1)z_n = 0$ reduces to $w^{2n+1} = -1$ (where $w \neq -1$ since $w \neq w'$). From this, $w = -\exp(\frac{-2pm\pi i}{2n+1})$, $p = 1, 2, \dots, n$. From now on we shall take this p as an index (i.e., use α_p , λ_p , μ_p , w_p , V_p , z_m^p , \mathbf{z}^p , x_m^p , \mathbf{x}^p).

The numbers and vectors α_p , λ_p , μ_p , w_p , V_p , x_m^p , \mathbf{x}^p are in fact those defined earlier. Normalization of $V_p \mathbf{z}^p$ yields the p th eigenvector \mathbf{x}^p as

$$x_m^p = 2(-1)^{m+1} \frac{\sin(2pm\pi/(2n+1))}{\sqrt{2n+1}}.$$

Similarly, one finds the formulas for α_p , λ_p etc.

The $\mathbf{x}^p(\alpha)$ form an orthogonal eigenbasis over which the symmetric matrix D^{-2} diagonalizes. But in fact by an easy calculation, $D^{-1}(\mathbf{x}^p)^T = \mu_p^{-1}(\mathbf{x}^p)^T$; hence D^{-1} and D diagonalize as well. This ends the proof. \square

Note that the eigenvalues μ_p of D are all different and $\max_p |\mu_p| = |\mu_n| = 1/2 \cos(n\pi/(2n+1))$. Also, $\text{sign } \mu_p = (-1)^{n+p}$ (consider $pn \bmod 2n+1$ for p odd and p even).

Corollary 2. *The (nonnegative integral) entries of D^k are given in closed form by the formula*

$$(D^k)_{i,j} = \sum_{p=1}^n (-1)^{i+j+(n+p)k} \frac{\sin(2pi\pi/(2n+1)) \sin(2pj\pi/(2n+1))}{(2n+1)2^{k-2} \cos^k(p\pi/(2n+1))}.$$

Proof. D^k can be written as $S\Delta^k S^T$ with $\Delta = \text{Diag}(\mu_1, \mu_2, \dots, \mu_n)$ and S the orthogonal basis transformation matrix having the $(\mathbf{x}^p)^T$'s as its columns. Thus, $(D^k)_{i,j} = \sum_{p=1}^n \mu_p^k x_i^p x_j^p$. \square

This also is the explicit solution of the recursion for the exponents vectors \mathbf{e}_i^k .

Remark 3. The following very nice graph-theoretic argument to find the eigenvalues of the matrix D was communicated by Blokhuis et al. [7].

Let $N = (-1)^n D^{-1}$. We can write $N = A - B$, where both A and B are 0–1 matrices (and A and B are zero wherever N is zero). With

$$P = \begin{pmatrix} A & B \\ B & A \end{pmatrix}$$

we see that P is the adjacency matrix of a path of length $2n$. Each eigenvector u of N with eigenvalue θ yields an antisymmetric eigenvector

$$\begin{pmatrix} u \\ -u \end{pmatrix}$$

of P with eigenvalue θ , and conversely. But the antisymmetric eigenvectors of P are precisely those that can be extended to eigenvectors of a $(2n+1)$ -cycle by defining it to be zero on the additional point. It follows that the eigenvalues are $\theta = 2 \cos(2\pi j/(2n+1))$, where $1 \leq j \leq n$ from which those of D follow. \square

4.2. The final estimate

In order to prove Corollary 1, we have to estimate the total degree of $\text{lt}(f)$. Let \mathbf{j} be the all-one column. By Theorem 1, there exists some nonzero column vector \mathbf{i} over $\mathbb{N} \cup \{0\}$ such that $\text{lt}(f) = \langle U D^{k-1} \mathbf{i}, \mathbf{j} \rangle = \langle D \mathbf{i}, D^{k-2} U^T \mathbf{j} \rangle = \langle D \mathbf{i}, D^{k-2} (1, 2, \dots, n)^T \rangle$. Note that $D \mathbf{i}$ has at least one positive entry, namely the n th. Hence,

$$\begin{aligned} \text{tdeg } f &\geq \sum_{q=1}^n q (D^{k-2})_{n,q} \\ &= \sum_{q=1}^n q \sum_{p=1}^n (-1)^{n+q+(n+p)k} \frac{\sin(2pn\pi/(2n+1)) \sin(2pq\pi/(2n+1))}{(2n+1)2^{k-2} \cos^k(p\pi/(2n+1))} \end{aligned}$$

by Corollary 2, putting $k - 2 = t$. Equality occurs if $\mathbf{i} = (1, 0, \dots, 0)^T$: e.g., if $f = a_1^k$.

The summation over the index q can easily, though tediously, be calculated explicitly (e.g, using the complex form of the sine or by computer algebra). The double sum then reduces to

$$\frac{(-1)^m}{(2n+1)2^t} \sum_{p=1}^n (-1)^p \frac{\sin(2pn\pi/(2n+1))^2}{\cos^{t+2}(p\pi/(2n+1))}.$$

Let H be the largest (n th) term; we shall see that it dominates. By Taylor expansion around $\pi/2$ one has, for some $|\theta| \leq 1$,

$$\sin\left(\frac{n\pi}{2n+1}\right) = 1 - \left(\frac{\pi}{2(2n+1)}\right)^2 \frac{\theta}{2!} \geq \frac{19}{20}. \quad (n \geq 2)$$

Similarly, $\cos(n\pi/2n+1) \leq \pi/2(2n+1)$. Thus,

$$H \geq \frac{4(2n+1)^{t+1}}{\pi^{t+2}} \left(\frac{19}{20}\right)^2.$$

Since $\cos x \geq 1 - (2x/\pi)$ on $[0, \pi/2]$, one has $\cos(p\pi/(2n+1)) \geq (2(n-p)+1)/(2n+1)$. Also, $\sin(2pn\pi/(2n+1))^2 \leq 1$. Hence, the sum of the absolute values of the first $n-1$ terms is not more than

$$\sum_{r=1}^{n-1} \frac{(2n+1)^{t+1}}{2^t(2r+1)^{t+2}}.$$

where $r = n - p$. However,

$$\sum_{r=1}^{n-1} \frac{1}{(2r+1)^{t+2}} \leq \frac{1}{3^{t+2}} + \int_1^n \frac{dx}{(2x+1)^{t+2}} \leq \frac{1}{3^{t+1}},$$

which yields the upper bound $\frac{(2n+1)^{t+1}}{2^t 3^{t+1}}$ for the small terms.

Combining this with our estimate for H we finally find

$$\text{tdeg}(f) \geq \frac{4(2n+1)^{t+1}}{\pi^{t+2}} \left(\frac{19}{20}\right)^2 - \frac{(2n+1)^{t+1}}{2^t 3^{t+1}}$$

from which Corollary 1 follows immediately. \square

5. An example of a “fixpoint polynomial”

In the introduction we mentioned the fixpoints of the iteration $(x_1, \dots, x_n) \rightarrow (a_1, \dots, a_n)$. An amusing and perhaps intriguing numerical example for $n = 4$ is the following:

$$\begin{aligned}
& (-T + 1)(-1.324717957T + 1)(0.7548776668T + 1) \\
& \times (0.5698402906T + 1) \approx 1 - 0.9999999994T \\
& - 1.324717957T^2 + 0.7548776668T^3 + 0.5698402912T^4
\end{aligned}$$

The relevant equations were solved in the obvious way using Maple, by first constructing a Groebner basis of the ideal $I(x_1 + x_2 + x_3 + x_4 - x_1, x_1x_2 + x_1x_3 + x_2x_3 + x_1x_4 + x_2x_4 + x_3x_4 - x_2, x_1x_2x_3 + x_1x_2x_4 + x_1x_3x_4 + x_2x_3x_4 - x_3, x_1x_2x_3x_4 - x_4)$.

Acknowledgements

I wish to thank A. Blokhuis, A.E. Brouwer and R. Riebeek for a stimulating discussion, and more in particular Andries Brouwer for his comments on a draft version of this article. I am also grateful to the (anonymous) referee for suggesting several improvements in the exposition and for the reference to Raney's work [5].

References

- [1] I.G. Macdonald, *Symmetric Functions and Hall Polynomials*, Oxford University Press, Oxford, 1979.
- [2] B.L. Van der Waerden, *Algebra*, vols. 1 and 2, Springer, Berlin, 1971.
- [3] J.H.-O. Peitgen, H. Jürgens, D. Saupe, *Fractals for the Classroom*, Springer, Berlin, 1992.
- [4] D. Cox, J. Little, D. O'Shea, *Ideals, Varieties and Algorithms*, Springer, Berlin, 1992.
- [5] G.N. Raney, Generalization of the Fibonacci sequence to n dimensions, *Canadian J. Math.* 18 (1966) 332–349.
- [6] T.S. Chihara, *An Introduction to Orthogonal Polynomials*, Gordon and Breach, London, 1978.
- [7] A. Blokhuis, A.E. Brouwer, R. Riebeek, private communication, Department of Mathematics, Eindhoven Techn. University, NL.